src/Trace.v
@@ -267,6 +267,14 @@ Inductive trace: AnnoTerm -> Plc -> Evidence ->
           ((Term_Defs.split (fst r) p)
              :: tr0 ++ tr1 ++
              [(join (pred (snd r)) p)])
+| tbpar: forall r s x y p e tr0 tr1 tr2,
+    trace x p (splitEv_T (fst s) e) tr0 ->
+    trace y p (splitEv_T (snd s) e) tr1 ->
+    shuffle tr0 tr1 tr2 ->
+    trace (abpar r s x y) p e
+          ((Term_Defs.split (fst r) p)
+             :: tr2 ++
+             [(join (pred (snd r)) p)])
           (*
 | tbpar: forall r lr s x y p tr0 tr1 tr2 (*xi xi'*) yi yi',
     trace x p tr0 ->
@@ -393,7 +401,34 @@ Proof.
       (*
       rewrite H10. *)
       apply evtsbseqjoin; auto.
+
+
       (*
+    +
+      inv_in; subst; try solve_by_inversion.
+      (*
+      
+
+      destruct H1; subst; try solve_by_inversion. *)
+      (*
+      apply evtsbseqsplit; auto. *)
+      rewrite in_app_iff in *; destruct_disjunct.
+      apply evtsbparl; auto.
+      rewrite in_app_iff in *; destruct_disjunct.
+      apply evtsbparr; auto.
+      inv_in; subst; try solve_by_inversion.
+      (*
+      destruct H0; subst; try solve_by_inversion. *)
+      repeat find_rewrite.
+      (*
+      rewrite H10. *)
+      apply evtsbparjoin; auto.
+*)
+
+
+
+      
+      
     +
       
 
@@ -426,7 +461,7 @@ Proof.
       rewrite H13 in H; simpl in H.
       destruct H; try tauto; subst. *)
       apply evtsbparjoin; auto. *)
-*)
+
   - induction H0; inv H.
     + inv H1; destruct r as [i j]; simpl in *; auto.
     + simpl; rewrite in_app_iff; simpl.
@@ -444,11 +479,26 @@ Proof.
       inv H1; auto.
       repeat find_rewrite.
       auto.
+
+
+      (*
+    + simpl.
+      rewrite in_app_iff.
+      rewrite in_app_iff.
+      simpl.
+      inv H1; auto.
+      repeat find_rewrite.
+      auto.
+       *)
+      
+
+
+      
       (*
       rewrite H12 in *.
       auto. *)
 
-      (*
+      
       
     + simpl.
       rewrite in_app_iff.
@@ -475,7 +525,6 @@ Proof.
       * apply IHtrace2 in H10; auto.
         eapply shuffle_in_right in H0; eauto.
       * repeat find_rewrite; simpl; auto. *)
-*)
 Qed.
 
 Lemma trace_range:
@@ -608,7 +657,7 @@ Proof.
       
     apply NoDup_cons.
     + intro.
-      repeat rewrite in_app_iff in *.
+      repeat rewrite in_app_iff in *;
       repeat destruct_disjunct;
         try solve_by_inversion.
       (*
@@ -721,9 +770,160 @@ Proof.
         lia.
         solve_by_inversion.
          *)
+
+
+
+
+
+(*
         
-     (*   
+
+  -
+    dest_range'; simpl in *; subst; simpl.
+    (*
+
+    destruct r as [i j]; simpl in *; subst; simpl. *)
+      
+    apply NoDup_cons.
+    + intro.
+      repeat rewrite in_app_iff in *.
+      repeat destruct_disjunct;
+        try solve_by_inversion.
+      (*
+        try (tr_wf;
+             simpl in *;
+             lia). *)
+
+      (*
+      *
+
+        (*
+        find_eapply_lem_hyp trace_range; eauto.
+        repeat find_rewrite.
+        simpl in *.
+         *)
         
+
+        (*
+        Locate tr_wf.
+
+        
+        repeat tr_wf.
+        simpl in *.
+        lia.
+
+        (*
+
+        eapply trace_range in H13; eauto.
+        simpl in H13.
+        lia. *)
+       *)
+       *)
+      
+
+      
+      *
+        repeat tr_wf.
+
+        (*
+
+        eapply trace_range in H14; eauto. *)
+        simpl in *.
+        Locate well_formed_range.
+        Check well_formed_range.
+        repeat find_eapply_lem_hyp well_formed_range_r; auto.
+
+
+        (*
+        apply well_formed_range_r in H6; auto.
+        lia. *)
+        simpl in *.
+        repeat tr_wf.
+        lia.
+      
+      * inv_in.
+        solve_by_inversion.
+        (*
+        discriminate H2.
+        solve_by_inversion. *)
+    + apply nodup_append; unfold disjoint_lists; auto; intros.
+      * eapply IHt1; eauto.
+      * apply nodup_append; unfold disjoint_lists; auto; intros;
+          try eauto;
+          try do_nodup;
+          try (inv_in; repeat tr_wf; simpl in *; lia).
+
+        (*
+        (*
+        -- eapply IHt2; eauto.
+         *)
+        
+        --
+          do_nodup.
+          (*
+
+          apply NoDup_cons.
+           intro HH; inv HH.
+           constructor. *)
+        --
+
+          inv_in.
+          repeat tr_wf.
+          simpl in *; lia.
+
+          (*
+          
+
+          inv H2.
+           eapply trace_range in H14; eauto.
+           simpl in H14.
+           lia.
+           solve_by_inversion. *)
+
+         *)
+
+
+        
+      *
+
+        rewrite in_app_iff in *; destruct_disjunct.
+
+        (*
+
+
+        apply in_app_iff in H2; destruct H2. *)
+
+        repeat tr_wf.
+        lia.
+
+        (*
+        
+        eapply trace_range in H13; eauto.
+        eapply trace_range in H14; eauto.
+        lia. *)
+
+        inv_in.
+        repeat tr_wf.
+        repeat find_eapply_lem_hyp well_formed_range_r; auto.
+        simpl in *.
+        lia.
+
+        (*
+
+        
+        inv H2.
+        eapply trace_range in H13; eauto.
+        simpl in H13.
+        apply well_formed_range_r in H7; auto.
+        lia.
+        solve_by_inversion.
+         *)
+
+*)
+
+        
+       
+      
   -
     dest_range'; simpl in *; subst; simpl.
     (*
@@ -747,11 +947,15 @@ Proof.
           try (tr_wf;
                simpl in *;
                lia).
-        (*
+        
         --
           tr_wf.
           simpl in *.
+          repeat find_eapply_lem_hyp well_formed_range_r; auto.
           lia.
+
+
+          (*
           (*
 
           eapply trace_range in H16; eauto.
@@ -831,7 +1035,6 @@ Proof.
 
         -- solve_by_inversion.
            *)
-*)
           
 Qed.
 
@@ -958,12 +1161,61 @@ Proof.
       repeat (rewrite in_app_iff; right).
       simpl; left; auto. *)
 
-      (*
+
+(*
+
       
+  - right.
+    rewrite in_app_iff in *.
+    do_evin; auto.
+
+    (*
+
+
+    inv H3; auto. *)
+    +
+      do_evin; auto;
+        eauto.
+      rewrite in_app_iff; auto.
+
+      (*
+
+      (*
+
+      inv H4; auto. *)
+      * apply IHtrace1 in H6; auto.
+        rewrite in_app_iff; auto.
+      * apply IHtrace2 in H7; auto.
+        rewrite in_app_iff.
+        right; rewrite in_app_iff; auto. *)
+    +
+      do_evin; auto.
+      (*
+      inv H4; auto. *)
+      (repeat rewrite in_app_iff; right).
+      right.
+      left.
+      auto.
+      (*
+      rewrite in_app_iff.
+      right.
+      simpl.
+      auto.
+      left.
+      simpl.
+      repeat (rewrite in_app_iff; right).
+      simpl; left; auto. *)
+
+*)
+
+      
+
+      
+      (*
   - left. solve_by_inversion.
        *)
 
-      (*
+      
       
   - right.
 
@@ -1008,7 +1260,6 @@ Proof.
       rewrite in_app_iff; right; simpl; auto.
       (*
       apply in_app_iff; right; simpl; auto. *)
-*)
 Qed.
 
 
@@ -1213,7 +1464,109 @@ Proof.
         apply earlier_left; auto.
     + solve_by_inversion.
 
+
+
       (*
+  -
+    do_evin2.
+    (*
+
+    inv H12; inv H11. *)
+    +
+      do_evin.
+      (*
+
+      inv H3. *)
+      *
+        find_eapply_lem_hyp evsys_tr_in; eauto.
+        (*
+
+        eapply evsys_tr_in in H4; eauto. *)
+        apply earlier_cons; auto.
+        apply in_app_iff; auto.
+      *
+        find_eapply_lem_hyp evsys_tr_in; eauto.
+        
+        apply earlier_cons; auto.
+        (*
+
+        
+        eapply evsys_tr_in in H4; eauto.
+        apply earlier_cons; auto. *)
+        apply in_app_iff; right;
+          apply in_app_iff; simpl; auto.
+    +
+      do_evin.
+      (*
+
+      inv H3. *)
+      apply earlier_cons; auto.
+      repeat (apply in_app_iff; right).
+      simpl; auto.
+  - solve_by_inversion.
+    
+  -
+    inv_prec.
+    (*
+
+    inv H11. *)
+    +
+      do_evin2.
+      (*
+
+      inv H13. inv H12. *)
+      *
+        find_eapply_lem_hyp evsys_tr_in; eauto.
+        (*
+
+        eapply evsys_tr_in in H3; eauto. *)
+        apply earlier_cons_shift; auto.
+        apply earlier_append; auto.
+        apply in_app_iff; right; simpl; auto.
+      *
+        find_eapply_lem_hyp evsys_tr_in; eauto.
+        (*
+
+        eapply evsys_tr_in in H3; eauto. *)
+        apply earlier_cons_shift; auto.
+        apply earlier_right; auto.
+        apply earlier_append; simpl; auto.
+    +
+      inv_prec.
+      (*
+
+      inv H12. *)
+      *
+        find_eapply_lem_hyp evsys_tr_in; eauto.
+        find_eapply_lem_hyp evsys_tr_in; eauto.
+
+        (*
+        eapply evsys_tr_in in H14; eauto.
+        eapply evsys_tr_in in H13; eauto. *)
+        apply earlier_cons_shift; auto.
+        apply earlier_append; auto.
+        apply in_app_iff; left; auto.
+      *
+        find_apply_hyp_hyp; auto.
+        (*
+
+        apply IHtrace1 in H6; auto. *)
+        apply earlier_cons_shift; auto.
+        apply earlier_left; auto.
+      *
+        find_apply_hyp_hyp; auto.
+        (*
+        apply IHtrace2 in H7; auto. *)
+        apply earlier_cons_shift; auto.
+        apply earlier_right; auto.
+        apply earlier_left; auto.
+    + solve_by_inversion.
+
+*)
+      
+
+      
+      
       
   -
     do_evin2.
@@ -1282,21 +1635,36 @@ Proof.
         apply shuffle_in_right with (e:=ev0) in H0; auto. *)
         apply earlier_cons_shift; auto.
         apply earlier_append; simpl; auto.
+
+
+
+        (*
     +
+
       inv_prec.
+      (*
+      find_eapply_lem_hyp shuffle_earlier_right; eauto. *)
+
+
+      
+      
       (*
       inv H9. *)
       *
-        find_apply_hyp_hyp; auto.
+        (*
+        find_apply_hyp_hyp; auto. *)
         find_eapply_lem_hyp shuffle_earlier_left.
         Focus 2.
         eauto.
+        eauto.
+        find_eapply_lem_hyp evsys_tr_in; eauto.
         (*
         apply IHtrace1 in H8; auto.
         apply shuffle_earlier_left
           with (e0:=ev0)(e1:=ev1) in H0; auto. *)
-        
-        apply earlier_cons_shift; auto.
+
+       (*
+        apply earlier_cons_shift; auto. *)
         apply earlier_left; auto.
       *
         find_apply_hyp_hyp; auto.
@@ -1311,6 +1679,8 @@ Proof.
           with (e0:=ev0)(e1:=ev1) in H0; auto. *)
         apply earlier_cons_shift; auto.
         apply earlier_left; auto.
+         *)
+
+    + admit.
     + solve_by_inversion.
-*)
-Qed.
+Admitted.
