src/MonadVM.v
@@ -79,17 +79,17 @@ Definition split_ev_seq (i:nat) (sp1 sp2:SP) (e:EvidenceC) (p:Plc) : CVM (Eviden
     let e2 := splitEv sp2 e in
     add_tracem [Term_Defs.split i p] ;;
     ret (e1,e2).
-(*
 
-Definition split_ev_par (i:nat) (sp1 sp2:SP) ((*loc_e1*) loc_e2:Loc)
+(*
+Definition split_ev_par (i:nat) (sp1 sp2:SP) (*((*loc_e1*) loc_e2:Loc) *)
            (*(t1 t2:AnnoTerm)*) (e:EvidenceC) (p:Plc) : CVM EvidenceC :=
     let e1 := splitEv sp1 e in
     let e2 := splitEv sp2 e in
     (*let loc_e1 := fst (range t1) in
     let loc_e2 := fst (range t2) in *)
     (*put_store_at loc_e1 e1 ;; *)
-    put_store_at loc_e2 e2 ;;
-    add_tracem [splitp i (*loc_e1*) loc_e2 p] ;;
+    (*put_store_at loc_e2 e2 ;; *)
+    add_tracem [Term_Defs.split i p] ;;
     ret e1.
 *)
 
@@ -193,14 +193,11 @@ Definition join_seq (n:nat) (p:Plc) (e1:EvidenceC) (e2:EvidenceC) : CVM unit :=
   put_ev (ssc e1 e2) ;;
   add_tracem [join n p].
 
-(*
-
-Definition join_par (n:nat) (p:Plc) (*(xi:Loc)*) (e1r:EvidenceC) (yi:Loc) (*(e1:EvidenceC) (e2:EvidenceC)*) : CVM unit :=
+Definition join_par (n:nat) (p:Plc) (*(xi:Loc)*) (e1r:EvidenceC) (e2r:EvidenceC) : CVM unit :=
   (*e1r <- get_store_at xi ;; *)
-  e2r <- get_store_at yi ;;
+  (*e2r <- get_store_at yi ;; *)
   put_ev (ppc e1r e2r) ;;
-  add_tracem [joinp n (*xi*) yi yi p].
-*)
+  add_tracem [join n p].
   
 
 (** * Helper functions for Appraisal *)
